theories/System/PGS.v
@@ -1,1 +1,17 @@
+Require Import PnV.Prelude.Prelude.
+Require Import PnV.Control.Monad.
+Require Import PnV.Data.FiniteMap.
+Require Import PnV.Data.FiniteSet.
+Require Import PnV.Data.Graph.
+Require Import PnV.System.Regex.
+Require Import Stdlib.Logic.Eqdep_dec.
 
+Import DoNotations.
+Import DigraphFixedpoint.
+
+#[local] Infix "\in" := E.In : type_scope.
+#[local] Infix "=~=" := (is_similar_to (Similarity := Re.in_regex eq)) : type_scope.
+#[local] Infix "∈" := L.In.
+#[local] Infix "⊑" := is_similar_to.
+
+#[local] Existing Instance Similarity_bool_Prop.
